veric/extend_tc.v
@@ -4,6 +4,8 @@ Require Import VST.veric.mpred.
 Require Import VST.veric.tycontext.
 Require Import VST.veric.expr2.
 Require Import VST.veric.binop_lemmas2.
+Require Import VST.veric.binop_lemmas4.
+Require Import VST.veric.expr_lemmas.
 
 Require Import VST.veric.seplog. (*For definition of tycontext*)
 Import LiftNotation.
@@ -12,7 +14,7 @@ Section mpred.
 
 Context `{!heapGS Σ}.
 
-Definition tc_expr {CS: compspecs} (Delta: tycontext) (e: expr) : environ -> mpred:=
+Definition tc_expr {CS: compspecs} (Delta: tycontext) (e: expr) : environ -> mpred :=
   fun rho => denote_tc_assert (typecheck_expr Delta e) rho.
 
 Definition tc_exprlist {CS: compspecs} (Delta: tycontext) (t : list type) (e: list expr) : environ -> mpred :=
@@ -27,459 +29,32 @@ Definition tc_temp_id {CS: compspecs} (id : positive) (ty : type)
 
 Definition tc_expropt {CS: compspecs} Delta (e: option expr) (t: type) : environ -> mpred :=
    match e with None => `⌜t=Ctypes.Tvoid⌝
-                     | Some e' => tc_expr Delta (Ecast e' t)
+                     | Some e' => `bi_absorbingly (tc_expr Delta (Ecast e' t))
    end.
 
 Definition tc_temp_id_load id tfrom Delta v : environ -> mpred  :=
 fun rho => ⌜exists tto, (temp_types Delta) !! id = Some tto
                       /\ tc_val tto (eval_cast tfrom tto (v rho))⌝.
 
-(*Lemma extend_prop: forall P, boxy extendM (prop P : mpred).
-Proof.
-intros.
-hnf.
-apply pred_ext. intros ? ?. apply H; auto. apply extendM_refl.
-repeat intro. apply H.
-Qed.
-
-#[export] Hint Resolve extend_prop : core.
-
-Lemma extend_tc_temp_id_load :  forall id tfrom Delta v rho, boxy extendM (tc_temp_id_load id tfrom Delta v rho).
-Proof.
-intros. unfold tc_temp_id_load. auto.
-Qed.
-
-Lemma extend_tc_andp:
- forall {CS: compspecs} A B rho,
-   boxy extendM (denote_tc_assert A rho) ->
-   boxy extendM (denote_tc_assert B rho) ->
-   boxy extendM (denote_tc_assert (tc_andp A B) rho).
-Proof.
-intros.
-rewrite denote_tc_assert_andp.
-apply boxy_andp; auto.
-intros ?; hnf.
-exists (core x); apply join_comm, core_unit.
-Qed.
-
-Lemma extend_tc_bool:
- forall {CS: compspecs} A B rho,
-   boxy extendM (denote_tc_assert (tc_bool A B) rho).
-Proof.
-intros.
-destruct A; simpl; apply  extend_prop.
-Qed.
-
-Lemma extend_tc_int_or_ptr_type:
- forall {CS: compspecs} A rho,
-   boxy extendM (denote_tc_assert (tc_int_or_ptr_type A) rho).
-Proof.
-intros.
-apply  extend_tc_bool.
-Qed.
-
-Lemma extend_tc_Zge:
- forall {CS: compspecs} v i rho,
-   boxy extendM (denote_tc_assert (tc_Zge v i) rho).
-Proof.
-intros.
-induction v; simpl; unfold_lift; simpl;
-unfold denote_tc_Zle; try apply extend_prop;
-repeat match goal with |- boxy _ (match ?A with  _ => _ end) => destruct A end;
-try apply extend_prop.
-Qed.
-
-Lemma extend_tc_Zle:
- forall {CS: compspecs} v i rho,
-   boxy extendM (denote_tc_assert (tc_Zle v i) rho).
-Proof.
-intros.
-induction v; simpl; unfold_lift; simpl;
-unfold denote_tc_Zge; try apply extend_prop;
-repeat match goal with |- boxy _ (match ?A with  _ => _ end) => destruct A end;
-try apply extend_prop.
-Qed.
-
-Lemma extend_tc_iszero:
- forall {CS: compspecs} v rho,
-   boxy extendM (denote_tc_assert (tc_iszero v) rho).
-Proof.
-intros.
-rewrite denote_tc_assert_iszero.
-destruct (eval_expr v rho); apply extend_prop.
-Qed.
-
-Lemma extend_valid_pointer':
-  forall a b, boxy extendM (valid_pointer' a b).
-Proof.
-intros.
-apply boxy_i; intros.
-apply extendM_refl.
-unfold valid_pointer' in *.
-simpl in *.
-destruct a; simpl in *; auto.
-forget (b0, Ptrofs.unsigned i + b) as p.
-destruct (w @ p) eqn:?H; try contradiction.
-destruct H as [w2 ?].
-apply (resource_at_join _ _ _ p) in H.
-rewrite H1 in H.
-inv H; auto.
-clear - H0 RJ.
-eapply join_nonidentity; eauto.
-destruct H as [w2 ?].
-apply (resource_at_join _ _ _ p) in H.
-rewrite H1 in H.
-inv H; auto.
-Qed.
-
-Lemma extend_andp: forall (P Q : mpred),
-  boxy extendM P -> boxy extendM Q -> boxy extendM (andp P Q).
-Proof.
- intros.
- apply boxy_i; intros.
- apply extendM_refl.
- destruct H2; split; eapply boxy_e; eauto.
-Qed.
-
-Lemma extend_orp: forall (P Q : mpred), 
-  boxy extendM P -> boxy extendM Q -> boxy extendM (orp P Q).
-Proof.
- intros.
- apply boxy_i; intros.
- apply extendM_refl.
- destruct H2; [left|right]; eapply boxy_e; eauto.
-Qed.
-
-Lemma extend_tc_test_eq:
-  forall {CS: compspecs} e1 e2 rho,
- boxy extendM (denote_tc_assert (tc_test_eq e1 e2) rho).
-Proof.
-intros.
-rewrite denote_tc_assert_test_eq'.
-apply boxy_i; intros.
-apply extendM_refl.
-simpl in *.
-super_unfold_lift.
-unfold denote_tc_test_eq in *.
-destruct (eval_expr e1 rho); auto;
-destruct (eval_expr e2 rho); auto.
-+ destruct H0; split; auto.
-  destruct H1 as [H1|H1]; [left|right];
-  apply (boxy_e _ _ (extend_valid_pointer' _ _) _ w' H H1).
-+ destruct H0; split; auto.
-  destruct H1 as [H1|H1]; [left|right];
-  apply (boxy_e _ _ (extend_valid_pointer' _ _) _ w' H H1).
-+
- unfold test_eq_ptrs in *.
- simple_if_tac;
- (eapply boxy_e;
-  [apply extend_andp; try apply extend_orp; apply extend_valid_pointer' | apply H | apply H0]).
-Qed.
-
-Lemma extend_tc_test_order:
-  forall {CS: compspecs} e1 e2 rho,
- boxy extendM (denote_tc_assert (tc_test_order e1 e2) rho).
-Proof.
-intros.
-rewrite denote_tc_assert_test_order'.
-apply boxy_i; intros.
-apply extendM_refl.
-simpl in *.
-super_unfold_lift.
-unfold denote_tc_test_order in *.
-destruct (eval_expr e1 rho); auto;
-destruct (eval_expr e2 rho); auto.
-+ unfold test_order_ptrs in *.
-  simple_if_tac; auto.
- eapply boxy_e;
-  [apply extend_andp; eapply extend_orp; apply extend_valid_pointer' | apply H | apply H0].
-Qed.
-
-Lemma extend_isCastResultType:
- forall {CS: compspecs} t t' v rho,
-   boxy extendM (denote_tc_assert (isCastResultType t t' v) rho).
-Proof.
-intros.
- unfold isCastResultType;
- destruct (classify_cast t t');
- repeat apply extend_tc_andp;
- try match goal with |- context [eqb_type _ _] => destruct (eqb_type t t') end;
- repeat match goal with
- | |- boxy _ (match ?A with  _ => _ end) => destruct A
- | |- boxy _ (denote_tc_assert (if ?A then _ else _) rho) => destruct A
- | |- boxy _ (denote_tc_assert (match t' with _ => _ end) rho) =>
-        destruct t' as [ | [ | | | ] [ | ] ? | [ | ] ? | [ | ] ? | | | | | ]
- end;
- repeat apply extend_tc_andp;
- try apply extend_prop;
- try simple apply extend_tc_bool;
- try simple apply extend_tc_Zge;
- try simple apply extend_tc_Zle;
- try simple apply extend_tc_iszero;
- try simple apply extend_tc_test_eq;
- try simple apply extend_tc_test_order.
-Qed.
-
-Lemma extend_tc_temp_id: forall {CS: compspecs} id ty Delta e rho, boxy extendM (tc_temp_id id ty Delta e rho).
-Proof.
-intros. unfold tc_temp_id. unfold typecheck_temp_id.
-destruct ((temp_types Delta) !! id) as [? | ];
- repeat apply extend_tc_andp;
- try apply extend_prop;
- try simple apply extend_tc_bool.
- apply extend_isCastResultType.
-Qed.
-
-Lemma extend_tc_samebase:
-  forall {CS: compspecs} e1 e2 rho,
-boxy extendM (denote_tc_assert (tc_samebase e1 e2) rho).
-Proof.
-intros.
-unfold denote_tc_assert; simpl.
-unfold_lift.
-destruct (eval_expr e1 rho), (eval_expr e2 rho);
-  apply extend_prop.
-Qed.
-
-Lemma extend_tc_nonzero:
- forall {CS: compspecs} v rho,
-   boxy extendM (denote_tc_assert (tc_nonzero v) rho).
-Proof.
-intros.
-rewrite denote_tc_assert_nonzero.
-destruct (eval_expr v rho); apply extend_prop.
-Qed.
-
-
-Lemma extend_tc_nodivover:
- forall {CS: compspecs} e1 e2 rho,
-   boxy extendM (denote_tc_assert (tc_nodivover e1 e2) rho).
-Proof.
-intros.
-rewrite denote_tc_assert_nodivover.
-destruct (eval_expr e1 rho); try apply extend_prop;
-destruct (eval_expr e2 rho); try apply extend_prop.
-Qed.
-
-Lemma extend_tc_nosignedover:
- forall op {CS: compspecs} e1 e2 rho,
-   boxy extendM (denote_tc_assert (tc_nosignedover op e1 e2) rho).
-Proof.
-intros.
-unfold denote_tc_assert.
-unfold_lift.
-destruct (typeof e1) as [ | _ [ | ] _ | | | | | | | ],
-       (typeof e2) as [ | _ [ | ] _ | | | | | | | ];
-unfold denote_tc_nosignedover;
-destruct (eval_expr e1 rho); try apply extend_prop;
-destruct (eval_expr e2 rho); try apply extend_prop.
-Qed.
-
-Lemma extend_tc_nobinover:
- forall op {CS: compspecs} e1 e2 rho,
-   boxy extendM (denote_tc_assert (tc_nobinover op e1 e2) rho).
-Proof.
-intros.
-unfold tc_nobinover.
-unfold if_expr_signed.
-destruct (typeof e1) as [ | _ [ | ] _ | [ | ] _ | | | | | | ],
-       (typeof e2) as [ | _ [ | ] _ | [ | ] _ | | | | | | ];
-      try apply extend_prop;
-destruct (eval_expr e1 any_environ); try apply extend_prop;
-destruct (eval_expr e2 any_environ); try apply extend_prop;
-try apply extend_tc_nosignedover.
-all:
-simple_if_tac; try apply extend_prop; try apply extend_tc_nosignedover.
-Qed.
-
-Lemma boxy_orp {A} `{H : ageable A}:
-     forall (M: modality) , reflexive _ (app_mode M) ->
-      forall P Q, boxy M P -> boxy M Q -> boxy M (P || Q).
-Proof.
-destruct M;
-intros.
-simpl in *.
-apply boxy_i; intros; auto.
-destruct H4; [left|right];
-eapply boxy_e; eauto.
-Qed.
-
-Lemma extend_tc_orp:
- forall {CS: compspecs} A B rho,
-   boxy extendM (denote_tc_assert A rho) ->
-   boxy extendM (denote_tc_assert B rho) ->
-   boxy extendM (denote_tc_assert (tc_orp A B) rho).
-Proof.
-intros.
-rewrite denote_tc_assert_orp.
-apply boxy_orp; auto.
-intros ?; eexists; apply join_comm, core_unit.
-Qed.
-
-
-Lemma extend_tc_ilt:
- forall {CS: compspecs} e i rho,
-   boxy extendM (denote_tc_assert (tc_ilt e i) rho).
-Proof.
-intros.
-rewrite denote_tc_assert_ilt'.
-simpl. unfold_lift.
-destruct (eval_expr e rho); try apply extend_prop.
-Qed.
-
-Lemma extend_tc_llt:
- forall {CS: compspecs} e i rho,
-   boxy extendM (denote_tc_assert (tc_llt e i) rho).
-Proof.
-intros.
-rewrite denote_tc_assert_llt'.
-simpl. unfold_lift.
-destruct (eval_expr e rho); try apply extend_prop.
-Qed.
-
-Lemma extend_tc_andp':
- forall {CS: compspecs} A B rho,
-   boxy extendM (denote_tc_assert A rho) ->
-   boxy extendM (denote_tc_assert B rho) ->
-   boxy extendM (denote_tc_assert (tc_andp' A B) rho).
-Proof.
-intros.
-apply boxy_andp; auto.
-intros ?; eexists; apply join_comm, core_unit.
-Qed.
-
-Ltac extend_tc_prover := 
+Ltac extend_tc_prover :=
   match goal with
-  | |- _ => solve [immediate]
-  | |- _ => apply extend_prop
-  | |- _ => first
-              [ simple apply extend_tc_bool
-              | simple apply extend_tc_int_or_ptr_type
-              | simple apply extend_tc_andp
-              | simple apply extend_tc_andp'
-              | simple apply extend_tc_Zge
-              | simple apply extend_tc_Zle
-              | simple apply extend_tc_iszero
-              | simple apply extend_tc_nonzero
-              | simple apply extend_tc_nodivover
-              | simple apply extend_tc_nobinover
-              | simple apply extend_tc_samebase
-              | simple apply extend_tc_ilt
-              | simple apply extend_tc_llt
-              | simple apply extend_isCastResultType
-              | simple apply extend_tc_test_eq
-              | simple apply extend_tc_test_order]
-  | |- boxy _ (denote_tc_assert (if ?A then _ else _) _) => destruct A
-  | |- boxy _ (denote_tc_assert match tc_bool ?A _ with _ => _ end _) =>
-             destruct A
-  | |- boxy _ (denote_tc_assert match ?A with Some _ => _ | None => _ end _) =>
-          destruct A
+  | |- _ => apply _
+  | |- Absorbing (if ?A then _ else _) => destruct A
+  | |- Absorbing (match ?A with _ => _ end) => destruct A
+  | |- Absorbing (match ?A with _ => _ end _) => destruct A
   end.
 
-Lemma extend_tc_binop: forall {CS: compspecs} Delta e1 e2 b t rho, 
-  boxy extendM (denote_tc_assert (typecheck_expr Delta e1) rho) ->
-  boxy extendM (denote_tc_assert (typecheck_expr Delta e2) rho) ->
-  boxy extendM (denote_tc_assert (isBinOpResultType b e1 e2 t) rho).
+Global Instance denote_tc_assert_absorbing : forall {CS: compspecs} a rho, Absorbing (denote_tc_assert a rho).
 Proof.
-intros.
-destruct b;
-unfold isBinOpResultType, tc_int_or_ptr_type, check_pp_int;
-match goal with
-| |- context [classify_add] => destruct (classify_add (typeof e1) (typeof e2)) eqn:C
-| |- context [classify_sub] => destruct (classify_sub (typeof e1) (typeof e2)) eqn:C
-| |- context [classify_cmp] => destruct (classify_cmp (typeof e1) (typeof e2)) eqn:C
-| |- context [classify_shift] => destruct (classify_shift (typeof e1) (typeof e2)) eqn:C
-| |- _ => idtac
-end;
-repeat extend_tc_prover;
-destruct (typeof e1) as [ | [ | | | ] [ | ] ? | [ | ] ? | [ | ] ? | | | | | ];
-destruct (typeof e2) as [ | [ | | | ] [ | ] ? | [ | ] ? | [ | ] ? | | | | | ];
-try inv C; try apply extend_prop;
-unfold binarithType, classify_binarith; repeat extend_tc_prover.
+  intros; induction a; simpl; try apply _; unfold_lift; rewrite /denote_tc_nonzero /denote_tc_iszero /denote_tc_test_eq /denote_tc_test_order
+    /denote_tc_igt /denote_tc_lgt /denote_tc_Zle  /denote_tc_Zge /denote_tc_nodivover /denote_tc_nosignedover /test_eq_ptrs /test_order_ptrs; repeat extend_tc_prover.
 Qed.
 
-Lemma extend_tc_expr: forall {CS: compspecs} Delta e rho, boxy extendM (tc_expr Delta e rho)
- with extend_tc_lvalue: forall {CS: compspecs} Delta e rho, boxy extendM (tc_lvalue Delta e rho).
-Proof.
-*
- clear extend_tc_expr.
- intros.
- unfold tc_expr.
- unfold tc_lvalue in extend_tc_lvalue.
-  induction e; simpl;
-  try pose proof (extend_tc_lvalue CS Delta e rho);
-  clear extend_tc_lvalue;
-try solve [
-  repeat extend_tc_prover;
-  try destruct t as [ | [ | | | ] [ | ] ? | [ | ] ? | [ | ] ? | | | | | ];
-  simpl;
-  repeat extend_tc_prover
- ].
- + (* unop *)
-   repeat extend_tc_prover.
-   destruct u; simpl; repeat extend_tc_prover;
-   destruct (typeof e) as [ | [ | | | ] [ | ] ? | [ | ] ? | [ | ] ? | | | | | ];
-   simpl; repeat extend_tc_prover.
-   unfold denote_tc_assert. unfold_lift. apply extend_tc_nosignedover.
-   unfold denote_tc_assert. unfold_lift. apply extend_tc_nosignedover.
-   unfold denote_tc_assert. unfold_lift. apply extend_tc_nosignedover.
-   unfold denote_tc_assert. unfold_lift. apply extend_tc_nosignedover.
-   unfold denote_tc_assert. unfold_lift. apply extend_tc_nosignedover.
- + repeat extend_tc_prover. eapply extend_tc_binop; eauto.
- + 
-  destruct t as [ | [ | | | ] [ | ] ? | [ | ] ? | [ | ] ? | | | | | ];
-  repeat extend_tc_prover;
-   destruct (typeof e) as [ | [ | | | ] [ | ] ? | [ | ] ? | [ | ] ? | | | | | ];
-   simpl; repeat extend_tc_prover.
-   destruct (field_offset (@cenv_cs CS) i (co_members c)) as [[? [|]] | ]; 
-  repeat extend_tc_prover.
-   destruct (union_field_offset (@cenv_cs CS) i (co_members c)) as [[[] [|]] | ]; 
-  repeat extend_tc_prover.
-   destruct (field_offset (@cenv_cs CS) i (co_members c0)) as [[? [|]] | ]; 
-  repeat extend_tc_prover.
-   destruct (union_field_offset (@cenv_cs CS) i (co_members c0)) as [[[] [|]] | ]; 
-  repeat extend_tc_prover.
-*
- clear extend_tc_lvalue.
- intros.
- unfold tc_expr in *.
- unfold tc_lvalue.
- induction e; simpl;
- try specialize (extend_tc_expr CS Delta e rho);
- repeat extend_tc_prover;
- destruct (typeof e) as [ | [ | | | ] [ | ] ? | [ | ] ? | [ | ] ? | | | | | ];
- simpl; repeat extend_tc_prover.
-   destruct (field_offset (@cenv_cs CS) i (co_members c)) as [[? [|]] | ]; 
-  repeat extend_tc_prover.
-   destruct (union_field_offset (@cenv_cs CS) i (co_members c)) as [[[] [|]] | ]; 
-  repeat extend_tc_prover.
-Qed.
-
-Lemma extend_tc_exprlist: forall {CS: compspecs} Delta t e rho, boxy extendM (tc_exprlist Delta t e rho).
-Proof.
- intros. unfold tc_exprlist.
-  revert e; induction t; destruct e; intros; simpl; auto;
-  try apply extend_prop.
- repeat apply extend_tc_andp; auto.
- apply extend_tc_expr.
- try simple apply extend_isCastResultType.
-Qed.
-
-Lemma extend_tc_expropt: forall {CS: compspecs} Delta e t rho, boxy extendM (tc_expropt Delta e t rho).
+Global Instance tc_expropt_absorbing: forall {CS: compspecs} Delta e t rho, Absorbing (tc_expropt Delta e t rho).
 Proof.
   intros. unfold tc_expropt.
-  destruct e.
-  + apply extend_tc_expr.
-  + apply extend_prop.
+  destruct e; apply _.
 Qed.
-
-Definition extendM_refl_rmap := @extendM_refl rmap _ _ _ _ _.
-
-#[export] Hint Resolve extend_tc_expr extend_tc_temp_id extend_tc_temp_id_load extend_tc_exprlist extend_tc_expropt extend_tc_lvalue : core.
-#[export] Hint Resolve extendM_refl_rmap : core.*)
-
-Require Import VST.veric.binop_lemmas4.
-Require Import VST.veric.expr_lemmas.
 
 Lemma tc_bool_i:
  forall {cs: compspecs} b e rho,
@@ -499,63 +74,6 @@ Section CENV_SUB.
  Proof. destruct a; simpl; auto. Qed.
 
 
-(*
-These all follow from denote_tc_assert_cenv_sub.
-
-  Lemma tc_nodivover'_cenv_sub a1 a2 rho:
-   denote_tc_assert(CS := CS) (tc_nodivover' a1 a2) rho ⊢
-   denote_tc_assert(CS := CS') (tc_nodivover' a1 a2) rho.
-  Proof.
-    by apply denote_tc_nodivover_eval_expr_cenv_sub.
-  Qed.
-
-
-  Lemma tc_samebase_cenv_sub a1 a2 rho:
-   denote_tc_assert(CS := CS) (tc_samebase a1 a2) rho ⊢
-   denote_tc_assert(CS := CS') (tc_samebase a1 a2) rho.
-  Proof.
-    simpl. unfold_lift.
-    iIntros "%"; iPureIntro.
-    revert H; apply istrue_sameblock_eval_expr_cenv_sub; auto.
-  Qed.
-
-
-  Lemma tc_nonzero'_cenv_sub a rho:
-   denote_tc_assert(CS := CS) (tc_nonzero' a) rho ⊢
-   denote_tc_assert(CS := CS') (tc_nonzero' a) rho.
-  Proof.
-    apply denote_tc_nonzero_eval_expr_cenv_sub; auto.
-  Qed.
-
-  Lemma tc_ilt'_cenv_sub a i rho:
-   denote_tc_assert(CS := CS) (tc_ilt' a i) rho ⊢
-   denote_tc_assert(CS := CS') (tc_ilt' a i) rho.
-  Proof.
-    simpl. unfold_lift.
-    destruct (Val.eq (@eval_expr CS a rho) Vundef).
-    rewrite e. simpl. iIntros "[]".
-    rewrite <- ?(eval_expr_cenv_sub_eq CSUB _ _ n).
-    auto.
-  Qed.
-
-  Lemma tc_llt'_cenv_sub a i rho:
-   denote_tc_assert(CS := CS) (tc_llt' a i) rho ⊢
-   denote_tc_assert(CS := CS') (tc_llt' a i) rho.
-  Proof.
-  simpl. unfold_lift.
-  destruct (Val.eq (@eval_expr CS a rho) Vundef).
-  rewrite e. simpl. iIntros "[]".
-  rewrite <- ?(eval_expr_cenv_sub_eq CSUB _ _ n).
-  auto.
-  Qed.
-
-  Lemma tc_test_eq'_cenv_sub a1 a2 rho:
-   denote_tc_assert(CS := CS) (tc_test_eq' a1 a2) rho ⊢
-   denote_tc_assert(CS := CS') (tc_test_eq' a1 a2) rho.
-  Proof.
-    apply denote_tc_test_eq_eval_expr_cenv_sub; auto.
-  Qed.*)
-
   Lemma tc_test_eq_cenv_sub a1 a2 rho:
    denote_tc_assert(CS := CS) (tc_test_eq(CS := CS) a1 a2) rho ⊢
    denote_tc_assert(CS := CS') (tc_test_eq(CS := CS') a1 a2) rho.
@@ -563,13 +81,6 @@ These all follow from denote_tc_assert_cenv_sub.
     rewrite !denote_tc_assert_test_eq'.
     apply denote_tc_assert_cenv_sub; auto.
   Qed.
-
-  (*Lemma tc_test_order'_cenv_sub a1 a2 rho:
-   denote_tc_assert(CS := CS) (tc_test_order' a1 a2) rho ⊢
-   denote_tc_assert(CS := CS') (tc_test_order' a1 a2) rho.
-  Proof.
-    apply denote_tc_test_order_eval_expr_cenv_sub; auto.
-  Qed.*)
 
 Lemma entails_refl : forall (P : mpred), P ⊢ P.
 Proof. done. Qed.
@@ -658,84 +169,6 @@ Proof.
   tc_expr_cenv_sub_tac; try apply (denote_tc_assert_cenv_sub CSUB).
 Qed.
 
-
-(*Lemma denote_tc_assert_andp_i:
-  forall x y rho w, 
-   denote_tc_assert x rho ⊢
-   denote_tc_assert y rho ⊢
-   denote_tc_assert (tc_andp x y) rho) w.
-Proof.
-intros.
-rewrite denote_tc_assert_andp. split; auto.
-Qed.
-
-Lemma denote_tc_assert_andp'_imp:
- forall x x' y y' rho w,
-  (denote_tc_assert(CS := CS x rho ⊢ denote_tc_assert(CS := CS' x' rho) w) ->
-  (denote_tc_assert(CS := CS y rho ⊢ denote_tc_assert(CS := CS' y' rho) w) ->
-  denote_tc_assert(CS := CS (tc_andp' x y) rho ⊢
-  denote_tc_assert(CS := CS' (tc_andp' x' y') rho) w.
-Proof.
-intros.
-destruct H1.
-split; auto.
-Qed.
-
-Lemma denote_tc_assert_andp_imp:
- forall x x' y y' rho w,
-  (denote_tc_assert(CS := CS x rho ⊢ denote_tc_assert(CS := CS' x' rho) w) ->
-  (denote_tc_assert(CS := CS y rho ⊢ denote_tc_assert(CS := CS' y' rho) w) ->
-  denote_tc_assert(CS := CS (tc_andp x y) rho ⊢
-  denote_tc_assert(CS := CS' (tc_andp x' y') rho) w.
-Proof.
-intros.
-rewrite @denote_tc_assert_andp in H1|-*.
-eapply denote_tc_assert_andp'_imp; eauto.
-Qed.
-
-Lemma denote_tc_assert_andp'_imp2:
- forall x x' y y' rho w,
-  (denote_tc_assert(CS := CS y rho ⊢ 
-   denote_tc_assert(CS := CS x rho ⊢ 
-   denote_tc_assert(CS := CS' x' rho) w) ->
-  (denote_tc_assert(CS := CS x rho ⊢
-   denote_tc_assert(CS := CS y rho ⊢
-   denote_tc_assert(CS := CS' y' rho) w) ->
-  denote_tc_assert(CS := CS (tc_andp' x y) rho ⊢
-  denote_tc_assert(CS := CS' (tc_andp' x' y') rho) w.
-Proof.
-intros.
-destruct H1.
-split; auto.
-Qed.
-
-Lemma denote_tc_assert_andp_imp2:
- forall x x' y y' rho w,
-  (denote_tc_assert(CS := CS y rho ⊢ 
-   denote_tc_assert(CS := CS x rho ⊢ 
-   denote_tc_assert(CS := CS' x' rho) w) ->
-  (denote_tc_assert(CS := CS x rho ⊢
-   denote_tc_assert(CS := CS y rho ⊢
-   denote_tc_assert(CS := CS' y' rho) w) ->
-  denote_tc_assert(CS := CS (tc_andp x y) rho ⊢
-  denote_tc_assert(CS := CS' (tc_andp x' y') rho) w.
-Proof.
-intros.
-rewrite @denote_tc_assert_andp in H1|-*.
-eapply denote_tc_assert_andp'_imp2; eauto.
-Qed.*)
-
-(*Lemma tc_bool_cenv_sub:
- forall b e rho,
-  denote_tc_assert(CS := CS) (tc_bool b e) rho ⊢
-  denote_tc_assert(CS := CS') (tc_bool b e) rho.
-Proof.
-intros.
-apply tc_bool_e in H.
-apply tc_bool_i.
-auto.
-Qed.*)
-
 Lemma tc_complete_type_cenv_sub:
  forall t e rho,
   denote_tc_assert(CS := CS) (tc_bool (complete_type (@cenv_cs CS) t) e) rho ⊢
@@ -746,52 +179,6 @@ unfold tc_bool.
 destruct (complete_type _ _) eqn: Hc; [|iIntros "[]"].
 rewrite (cenv_sub_complete_type _ _ CSUB); auto.
 Qed.
-
-(*Local Lemma tc_andp'_intro:
-  forall x y rho w Q P,
-   (denote_tc_assert(CS := CS x rho ⊢
-    denote_tc_assert(CS := CS y rho ⊢
-    Q -> P) ->
-   (denote_tc_assert(CS := CS (tc_andp' x y) rho ⊢ Q -> P).
-Proof.
-intros.
-destruct H; auto.
-Qed.
-
-Local Lemma tc_andp_intro:
-  forall x y rho w Q P,
-   (denote_tc_assert(CS := CS x rho ⊢
-    denote_tc_assert(CS := CS y rho ⊢
-    Q -> P) ->
-   (denote_tc_assert(CS := CS (tc_andp x y) rho ⊢ Q -> P).
-Proof.
-intros.
-rewrite @denote_tc_assert_andp in H.
-destruct H; auto.
-Qed.
-
-Local Lemma tc_bool_intro:
-  forall b e rho w Q P,
-   (b = true -> Q -> P) ->
-   (denote_tc_assert(CS := CS (tc_bool b e) rho ⊢ Q -> P).
-Proof.
-intros.
-apply tc_bool_e in H. auto.
-Qed.
-
-Lemma tc_check_pp_int'_cenv_sub:
- forall a1 a2 op t e rho w,
- denote_tc_assert(CS := CS (check_pp_int' a1 a2 op t e) rho ⊢
- denote_tc_assert(CS := CS' (check_pp_int' a1 a2 op t e) rho) w.
-Proof.
-unfold check_pp_int'.
-intros.
-destruct op; try contradiction H; revert H;
- (apply denote_tc_assert_andp'_imp; 
-  [ | apply tc_bool_cenv_sub]).
-all: try simple apply tc_test_eq'_cenv_sub.
-all: try simple apply tc_test_order'_cenv_sub.
-Qed.*)
 
 Lemma tc_expr_cenv_sub_binop:
  forall 
